# HW10

## 1

$\textbf{Calculation not guaranteed.}$
(a)
$\mathcal{L}(\boldsymbol{x}, \boldsymbol{\lambda})=\boldsymbol{x^TA^TAx}-2\boldsymbol{b^TAx}+\boldsymbol{b^Tb}+\boldsymbol{\lambda}^T(\boldsymbol{Gx}-\boldsymbol{h})
$
$$
\nabla\mathcal{L}(\boldsymbol{x}, \boldsymbol{\lambda})=0\Rightarrow
\begin{bmatrix}
2A^TA & G^T\\
G & 0
\end{bmatrix}
\begin{bmatrix}
\boldsymbol{x}\\
\boldsymbol{\lambda}
\end{bmatrix}=
\begin{bmatrix}
2A^Tb\\
h
\end{bmatrix}
$$

(b)
$\boldsymbol{x}^*=(A^TA)^{-1}(A^Tb-(G(A^TA)^{-1}G^T)^{-1}(G(A^TA)^{-1}A^Tb-h))$
$\boldsymbol{\lambda}^*=2(G(A^TA)^{-1}G^T)^{-1}(G(A^TA)^{-1}A^Tb-h)$

(c)
$x^*=...,\lambda^*=...$

(d)
$$
\begin{aligned}
\min_{\boldsymbol{z}}\quad g(\boldsymbol{z})=\Vert A(\boldsymbol{Fz}+\tilde{\boldsymbol{x}})-b\Vert^2
\end{aligned}
$$
$
where\ X=\{x|Gx=h\}=\{\tilde{x}+Fz|z\in\mathbb{R}^{n-k}\}
,F=\begin{bmatrix}
1 \\
-1
\end{bmatrix},
\tilde{x}=\begin{bmatrix}
1\\
0
\end{bmatrix}
$
$Therefore,z^*=\frac{11}{6} ,x^*=\begin{bmatrix}
\frac{17}{6}\\
-\frac{11}{6}
\end{bmatrix}$

## 2

(a)
$$
\begin{aligned}
\min_{\boldsymbol{d}}\quad &h(d)\triangleq f(x_0)+(Ax_0-b)^TQ(Ax_0-b)+(\nabla f(x_0) + 2A^TQ(Ax_0-b))^Td+\frac{1}{2}d^T(\nabla^2f(x_0)+2A^TQA)d\\
s.t.\quad & Ad=0
\end{aligned}
$$

KKT system:
$$
\begin{bmatrix}
\nabla^2f(x_0) & A^T\\
A & 0
\end{bmatrix}
\begin{bmatrix}
d\\
\lambda
\end{bmatrix}=
\begin{bmatrix}
-\nabla f(x_0)\\
0
\end{bmatrix}
$$

(b)
KKT system for (1):
$$
\begin{bmatrix}
\nabla^2f(x_0) & A^T\\
A & 0
\end{bmatrix}
\begin{bmatrix}
d\\
\lambda
\end{bmatrix}=
\begin{bmatrix}
-\nabla f(x_0)\\
0
\end{bmatrix}
$$
$d\ and\ \lambda\ are\ the\ same.$

## 3

(a)
$
\mathcal{L}(x,\lambda)=f(x)+\lambda(\boldsymbol{1}^Tx-1)
$
$$
\nabla\mathcal{L}(x,\lambda)=0\Rightarrow
x^*=\begin{bmatrix}
\frac{1+\ln2}{2}\\
\frac{1-\ln2}{4}\\
\frac{1-\ln2}{4}
\end{bmatrix}
,\lambda^*=-\sqrt{2}e^{\frac{1}{2}},f^*=3\sqrt{2}e^{\frac{1}{2}}
$$

$(b)$
$$
\begin{aligned}
\min_{x}\quad &h(d)\triangleq e^{x_1}+e^{2x_2}+e^{2x_3}+\begin{bmatrix}
e^{x_1}\\
2e^{2x_2}\\
2e^{2x_3}
\end{bmatrix}^Td+\frac{1}{2}d^T\begin{bmatrix}
e^{x_1} & 0 & 0\\
0 & 4e^{2x_2} & 0\\
0 & 0 & 4e^{2x_3}
\end{bmatrix}d\\
\textrm{s.t.}\quad &\boldsymbol{1}^Td=0\\
\end{aligned}
$$
$Therefore\ d\ = \begin{bmatrix}
1-d_2-d_3\\
\frac{\frac{9}{4}-\frac{1}{4}e^{2x_2-2x_3}-e^{3x_2+x_3-1}}{e^{2x_2-2x_3}+4e^{3x_2+x_3-1}+1}\\
\frac{\frac{9}{4}-\frac{1}{4}e^{2x_3-2x_2}-e^{3x_3+x_2-1}}{e^{2x_3-2x_2}+4e^{3x_3+x_2-1}+1}
\end{bmatrix}$
