# HW13

## 1

$(a)$
$x^*=(1,0), f^*=1$

$(b)$
$The\ Lagrange\ function\ is$
$$
\mathcal{L}(x, \mu)=x_1^2+x_2^2+\mu_1((x_1-1)^2+(x_2-1)^2-1)+\mu_2((x_1-1)^2+(x_2+1)^2-1)
$$
$The\ Lagrange\ dual\ function\ is$
$$
\phi(\mu)=\inf_{x}\mathcal{L}(x, \mu)=\begin{cases}
-\frac{2\mu_1^2+2\mu_2^2}{\mu_1+\mu_2+1}+\mu_1+\mu_2&, \mu_1+\mu_2+1> 0\\
-\infty&, \mu_1+\mu_2+1\leq 0
\end{cases}
$$
$The\ dual\ problem\ is$
$$
\begin{aligned}
\max_{\mu}&\quad-\frac{2\mu_1^2+2\mu_2^2}{\mu_1+\mu_2+1}+\mu_1+\mu_2\\
\textrm{s.t.}&\quad\mu_1+\mu_2+1> 0\\
\end{aligned}
$$
$Therefore\ \mu_1^*=\mu_2^*\rightarrow+\infty,\ \phi^*=1$

$(c)$
$Slater's\ condition\ does\ not\ hold.\ Thus\ Slater's\ condition\ is\ not\ necessary\ for\ strong\ duality.$

$(d)$

$\phi^*\ can\ not\ be\ attanied\ by\ feasible\ point.$
$KKT\ conditions:$
$$
\begin{cases}
\nabla_x\mathcal{L}(x^*, \mu^*)=0\\
\mu_1^*((x_1^*-1)^2+(x_2^*-1)^2-1)=0\\
\mu_2^*((x_1^*-1)^2+(x_2^*+1)^2-1)=0\\
(x_1^*-1)^2+(x_2^*-1)^2-1\leq 0\\
(x_1^*-1)^2+(x_2^*+1)^2-1\leq 0\\
\mu_1^*\geq 0\\
\mu_2^*\geq 0\\
\end{cases}
$$
$Substitute\ x^*=(1,0),\ we\ can\ find\ there\ are\ no\ Lagrange\ multipliers\ satisfying\ the\ KKT\ conditions\ at\ x^*.$
$\textbf{Tip:}\ After\ validation,\ x^*\ is\ not\ a\ regular\ point.\ So\ KKT\ conditions\ do\ not\ need\ to\ be\ satisfied\ here. $

## 2

$(a)$
$$
\begin{aligned}
\phi(\mu)&=\inf_{x\succeq0}\mathcal{L}(x, \mu)\\
&=\inf_{x\succeq0}x_1^3+x_2^3+\mu(1-x_1-x_2)\\
&=\inf_{x_1\geq 0}(x_1^3-\mu x_1)+\inf_{x_2\geq 0}(x_2^3-\mu x_2)+\mu\\
&=\begin{cases}
\mu&, \mu\leq 0\\
\frac{-4}{3\sqrt{3}}\mu^{\frac{3}{2}}+\mu&, \mu>0
\end{cases}
\end{aligned}
$$

$(b)$
$Notice\ that\ \phi^*\ is\ attained\ at\ \mu > 0$
$$
\begin{aligned}
\phi^*&=\sup_{\mu\geq 0}\phi(\mu)\\
&=\sup_{\mu>0}\frac{-4}{3\sqrt{3}}\mu^{\frac{3}{2}}+\mu\\
&=\frac{1}{4}
\end{aligned}
$$

$(c)$
$KKT\ conditions:$
$$
\begin{cases}x_1^*+x_2^*\geq1\\
\nabla_x\mathcal{L}(x^*, \mu^*)=0\\
\mu^*\geq 0\\
\mu^*(1-x_1^*-x_2^*)=0\\
x_1^*\geq 0\\
x_2^*\geq 0\\
\end{cases}\Rightarrow
\begin{cases}
x_1^*=\frac{1}{2}\\
x_2^*=\frac{1}{2}\\
\mu^*=\frac{3}{4}
\end{cases}
$$
$f^*=f(\frac{1}{2}, \frac{1}{2})=\frac{1}{4}$

$(d)$
$The\ dual\ function\ of\ (P2)\ is$
$$
\begin{aligned}
\phi(\mu)&=\inf_{x}\mathcal{L}(x, \mu)\\
&=\inf_{x}x_1^3+x_2^3+\mu(1-x_1-x_2)\\
&=\inf_{x_1}(x_1^3-\mu x_1)+\inf_{x_2}(x_2^3-\mu x_2)+\mu\\
&=-\infty
\end{aligned}
$$
$Strong\ duality\ does\ not\ hold.$
$\textbf{Tip:}\ f\ is\ not\ convex\ in\ \mathbb{R}^2,\ the\ problem\ does\ not\ apply\ to\ Slater's\ condition.$
